

Вариант 10

$$X = \frac{(p^2 - \frac{1}{q^2})^p (p - \frac{1}{q})^{q-p}}{(q^2 - \frac{1}{p^2})^q (q - \frac{1}{p})^{p-q}} \quad (1)$$

$$\begin{cases} \frac{y}{4} - \frac{x}{5} = 6 \\ \frac{x}{15} + \frac{y}{12} = 0 \end{cases} \quad (2)$$

$$\oint_r 2x dx - dy + 4dz \quad (3)$$

$$\sum_{n=1}^{\infty} \frac{2n-3}{5n+1} \quad (4)$$

$$\lim_{x \rightarrow 3} \frac{x^2 + x + 2}{x^2 + 2x + 8} = \frac{14}{23} \quad (5)$$

$$A^{-1} = -\frac{1}{2} \begin{pmatrix} 4 & -3 \\ -2 & 1 \end{pmatrix} \quad (6)$$